coq-SystemRF-3.1/Bidirectional/SynthFType.v
@@ -1,0 +1,831 @@
+Require Import SystemRF.BasicDefinitions. 
+Require Import SystemRF.Names.
+Require Import SystemRF.BasicPropsEnvironments.
+Require Import SystemRF.SystemFWellFormedness.
+Require Import SystemRF.SystemFTyping.
+Require Import SystemRF.Typing.
+Require Import Bidirectional.Decidable.
+Require Import Bidirectional.SynthWFFT.
+
+From Equations Require Import Equations.
+
+Require Import Arith.
+Require Import ZArith.
+
+Fixpoint edepth (e : expr) : nat :=
+    match e with 
+    | (Bc b)          => 0
+    | (Ic n)          => 0
+    | (Prim c)        => 0
+    | (BV i)          => 0
+    | (FV x)          => 0
+    | (Lambda e)      => 1 + (edepth e)
+    | (App e1 e2)     => 1 + max (edepth e1) (edepth e2)
+    | (LambdaT k e)   => 1 + (edepth e)
+    | (AppT e t)      => 1 + (edepth e)
+    | (Let ex e)      => 1 + max (edepth ex) (edepth e)
+    | (Annot e t)     => 1 + (edepth e)
+    | (If e0 e1 e2)   => 1 + max (edepth e0) (max (edepth e1) (edepth e2))
+    | Nil _           => 0
+    | (Cons _ e1 e2)  => 1 + max (edepth e1) (edepth e2)
+    | (Switch e eN eC) => 1 + max (edepth e) (max (edepth eN) (edepth eC))
+    | Error           => 0
+    end.
+
+Lemma edepth_open_at : forall (j:index) (y:vname) (e:expr),
+    edepth (open_at j y e) = edepth e.
+Proof. intros j y e; revert j; induction e; intros;
+  simpl; try destruct (Nat.eqb j i); reflexivity || f_equal;
+  apply IHe || f_equal; try apply f_equal2; 
+  apply IHe1 || apply IHe2 || apply IHe3. Qed.
+
+Lemma edepth_unbind : forall (y:vname) (e:expr),
+    edepth (unbind y e) = edepth e.
+Proof. intros; apply edepth_open_at; assumption. Qed.
+
+Lemma edepth_open_tv_at : forall (j:index) (a:vname) (e:expr),
+    edepth (open_tv_at j a e) = edepth e.
+Proof. intros j a e; revert j; induction e; intros;
+  simpl; try destruct (Nat.eqb j i); reflexivity || f_equal;
+  apply IHe || f_equal; try apply f_equal2; 
+  apply IHe1 || apply IHe2 || apply IHe3. Qed.
+
+Lemma edepth_unbind_tv : forall (a:vname) (e:expr),
+    edepth (unbind_tv a e) = edepth e.
+Proof. intros; apply edepth_open_tv_at; assumption. Qed.
+
+
+(*** we need a stack env for BV deBruijn's and their ftypes ***)
+
+Inductive deBruijnsF : Set := 
+    | DFEmpty 
+    | DFBind  (t : ftype) (d : deBruijnsF).
+
+Fixpoint bv_bound_inF (i : index) (t : ftype) (d : deBruijnsF) : Prop :=
+    match d with 
+    | DFEmpty      => False
+    | DFBind t' d' => match i with
+                      | 0     => t = t'
+                      | (S j) => bv_bound_inF j t d'
+                      end
+    end.      
+
+Fixpoint lookupDF (i : index) (d : deBruijnsF) : option ftype :=
+    match d with 
+    | DFEmpty      => None
+    | DFBind t' d' => match i with
+                      | 0     => Some t'
+                      | (S j) => lookupDF j d'
+                      end
+    end.
+
+Lemma lem_lookupDF_bvboundinF : 
+  forall (d : deBruijnsF) (i : index) (t : ftype) ,
+    lookupDF i d = Some t -> bv_bound_inF i t d.
+Proof. induction d; intros; destruct i;
+  simpl in H; try discriminate; simpl.
+  - injection H as H; auto.
+  - apply IHd; trivial.
+Qed.
+
+Fixpoint dflen (d : deBruijnsF) : nat :=
+    match d with
+    | DFEmpty       => 0
+    | (DFBind t d') => dflen d' + 1
+    end.    
+
+Lemma lem_bvboundinF_upper_bound : forall (i:index) (t:ftype) (d:deBruijnsF),
+    bv_bound_inF i t d -> i < dflen d.
+Proof. induction i; intros; destruct d; try contradiction.
+  - (* Base *) simpl; auto with *.
+  - (* Ind *) simpl. rewrite <- plus_n_Sm; rewrite <- plus_n_O; auto with *.
+  Qed.
+
+Fixpoint concatDF (d d'0 : deBruijnsF) : deBruijnsF :=
+    match d'0 with
+    | DFEmpty       => d
+    | (DFBind t d') => DFBind t (concatDF d d')
+    end.    
+
+Lemma lem_empty_concatDF : forall (d : deBruijnsF),
+    concatDF DFEmpty d = d.
+Proof. induction d; simpl; try rewrite IHd; reflexivity. Qed.    
+
+Lemma lem_bvboundinF_append : forall (d : deBruijnsF) (i:index) (t t':ftype),
+    bv_bound_inF i t (concatDF (DFBind t' DFEmpty) d) 
+          ->   i < dflen d /\ bv_bound_inF i t d
+            \/ i = dflen d /\ t = t'.
+Proof. induction d; intros.
+  - (* Base *) destruct i; simpl in H; right; intuition;
+    destruct i; try contradiction.
+  - (* Ind *) destruct i; simpl in H. 
+      * (* 0 *) subst t0; simpl; left; auto with *.
+      * (* S i *) apply IHd in H; destruct H; [left|right].
+          + (* in d *) destruct H; split; simpl; auto with *.
+          + (* at end *) simpl; rewrite <- plus_n_Sm; rewrite <- plus_n_O;
+            destruct H; split; auto.
+  Qed.
+
+
+Fixpoint lookupF (x : vname) (g : fenv) : option ftype :=
+    match g with 
+    | FEmpty          => None
+    | FCons x' t' g'  => if (x =? x') then Some t' else lookupF x g'
+    | FConsT a' k' g' => lookupF x g'
+    end.
+    
+Lemma lem_lookupF_boundinF : 
+  forall (g : fenv) (x : vname) (t : ftype) ,
+    lookupF x g = Some t -> bound_inF x t g.
+Proof. induction g; intros; 
+  simpl in H; try discriminate; simpl.
+  - destruct (x0 =? x) eqn:X.
+    * left; injection H as H; split; apply Nat.eqb_eq in X; auto.
+    * right; apply IHg; apply H.
+  - apply IHg; apply H.
+Qed.
+
+
+(*----------------------------------------------------------------------------
+  --- | AUTOMATED INFERENCE of SYSTEM F TYPING JUDGMENTS
+  --------------------------------------------------------------------------*)
+
+(* one version is computable function, the other is a mutually inductive
+      prop that we prove is decidable using the first way *)
+
+(* For the checkF'/synthF' functions, we can't use mutual recursion directly
+      because the argument e isn't strictly decreasing: in one case
+      `checkF' ... e` calls `synthF' ... e` but never vice-versa. One
+      solution would be to use mutual well-founded recursion, but Equations
+      does not suppor that yet. The remaining solution is to combine both
+      into one function: *)
+
+Inductive modeF : Set := ChkF (t : ftype) | SynF.
+
+Definition modeFsize (m : modeF) : nat :=
+  match m with 
+  | ChkF _ => 1
+  | SynF   => 0
+  end.
+
+Inductive resultF : modeF -> Set :=
+    | resF_Chk : forall (b : bool) (t:ftype), resultF (ChkF t)
+    | resF_Syn : forall ot : option ftype, resultF SynF.
+
+(* It would be nice to write this as Fixpoints, however the last
+    case in synthF' makes termination too tricky w/o Equations*)
+Equations bidirCheckF' (g:fenv) (df:deBruijnsF) (dtv:deBruijnTVs) 
+                       (e:expr) (m : modeF) : resultF m 
+  by wf (edepth e, modeFsize m) (lexprod _ _ lt lt ) :=
+(* checkF' definitions *)
+bidirCheckF' g df dtv (Lambda e') (ChkF t)    := 
+    match t with
+    | (FTFunc tx t')  => 
+        match bidirCheckF' g (DFBind tx df) dtv e' (ChkF t') with
+        | resF_Chk b _t' => resF_Chk (isWFFTb' g dtv tx Star 
+                                        && ftype_eq t' _t' && b ) t
+        | _              => resF_Chk false t
+        end
+    | _               => resF_Chk false t
+    end;
+bidirCheckF' g df dtv (LambdaT k e') (ChkF t) :=
+    match t with
+    | (FTPoly k' t')  => 
+        match bidirCheckF' g df (DTBind k dtv) e' (ChkF t') with
+        | resF_Chk b _t' => resF_Chk (kind_eq k k' 
+                                        && ftype_eq t' _t' && b) t
+        | _              => resF_Chk false t
+        end
+    | _               => resF_Chk false t
+    end;
+bidirCheckF' g df dtv (Let e_x e') (ChkF t)   :=
+    match bidirCheckF' g df dtv e_x SynF with
+    | resF_Syn (Some t_x)    => bidirCheckF' g (DFBind t_x df) dtv e' (ChkF t) 
+    (*| resF_Syn None          => resF_Chk false t*)
+    | _                      => resF_Chk false t
+    end;
+bidirCheckF' g df dtv (If e0 e1 e2) (ChkF t)  := 
+    match bidirCheckF' g df dtv e0 (ChkF (FTBasic TBool)) with
+    | resF_Chk b _ =>
+        match bidirCheckF' g df dtv e1 (ChkF t) with
+        | resF_Chk b' _ => 
+            match bidirCheckF' g df dtv e2 (ChkF t) with
+            | resF_Chk b'' _ => resF_Chk (b && b' && b'') t
+            | _              => resF_Chk false t
+            end
+        | _             => resF_Chk false t
+        end
+    | _ => resF_Chk false t
+    end;
+bidirCheckF' g df dtv (Switch e eN eC) (ChkF t) := 
+    match ( bidirCheckF' g df dtv e SynF ) with
+    | resF_Syn (Some (FTList t0)) => 
+        match bidirCheckF' g df dtv eN (ChkF t) with
+        | resF_Chk b _ =>
+            match bidirCheckF' g df dtv eC 
+                               (ChkF (FTFunc t0 (FTFunc (FTList t0) t))) with
+            | resF_Chk b' _ => resF_Chk (b && b') t
+            | _             => resF_Chk false t
+            end
+        | _            => resF_Chk false t
+        end
+    (*| resF_Syn _                  => resF_Chk false t     *)
+    | _                           => resF_Chk false t  
+    end;
+bidirCheckF' g df dtv e (ChkF t') :=
+    match (bidirCheckF' g df dtv e SynF) with
+    | resF_Syn (Some t'') => resF_Chk (ftype_eq t' t'') t'
+                                (* no subtypes: exact match only *)
+    (*| resF_Syn None       => resF_Chk false t'*)
+    | _                   => resF_Chk false t'
+    end;
+(* synthF' definitions *)
+bidirCheckF' g df dtv (Bc b) SynF      := resF_Syn (Some ( FTBasic TBool ));
+bidirCheckF' g df dtv (Ic n) SynF      := resF_Syn (Some ( FTBasic TInt ));
+bidirCheckF' g df dtv (Prim c) SynF    := resF_Syn (Some ( erase_ty c ));
+bidirCheckF' g df dtv (BV i) SynF      := resF_Syn (lookupDF i df);
+bidirCheckF' g df dtv (FV x) SynF      := resF_Syn (lookupF x g);
+bidirCheckF' g df dtv (App e e') SynF  := 
+    match ( bidirCheckF' g df dtv e SynF ) return (resultF SynF) with
+    | resF_Syn (Some (FTFunc t_x t)) =>
+        match ( bidirCheckF' g df dtv e (ChkF t_x) ) 
+            return (resultF SynF) with
+        | resF_Chk true  _t => resF_Syn (Some t)
+        | resF_Chk false _ => resF_Syn None 
+        | _                => resF_Syn None
+        end
+    | resF_Syn _                     => resF_Syn None
+    | _                              => resF_Syn None
+    end;
+bidirCheckF' g df dtv (AppT e' rt) SynF :=
+    match ( bidirCheckF' g df dtv e' SynF ) with
+    | resF_Syn (Some (FTPoly k s))   =>  
+        if (  isMonob rt && noExistsb rt          &&
+              isLCT_atb (dflen df) (dtlen dtv) rt &&
+              Subsetb (free rt) (vbindsF g)       && 
+              Subsetb (freeTV rt) (tvbindsF g)    &&
+              isWFFTb' g dtv (erase rt) Star )%bool
+        then resF_Syn (Some (ftsubBV (erase rt) s))
+        else resF_Syn None
+    (*| resF_Syn _                   => resF_Syn None *)
+    | _                            => resF_Syn None
+    end ;
+bidirCheckF' g df dtv (Annot e' rt) SynF :=
+    match ( bidirCheckF' g df dtv e' (ChkF (erase rt)) ) with
+    | resF_Chk true  _ => 
+        if ( isLCT_atb (dflen df) (dtlen dtv) rt &&
+             Subsetb (free rt) (vbindsF g)       &&
+             Subsetb (freeTV rt) (tvbindsF g) )%bool
+        then resF_Syn (Some (erase rt))
+        else resF_Syn None
+    (*| resF_Chk false _ => resF_Syn None*)
+    | _                => resF_Syn None
+    end;
+bidirCheckF' g df dtv (Nil t) SynF        := 
+    if isWFFTb' g dtv (erase t) Star
+    then resF_Syn (Some (FTList (erase t)))
+    else resF_Syn None;
+bidirCheckF' g df dtv (Cons t eH eT) SynF :=
+    match bidirCheckF' g df dtv eH (ChkF (erase t)) with 
+    | resF_Chk true  _  => 
+        match bidirCheckF' g df dtv eT (ChkF (FTList (erase t))) with
+        | resF_Chk true  _ => resF_Syn (Some (FTList (erase t) ))
+        | resF_Chk false _ => resF_Syn None 
+        | _                => resF_Syn None
+        end
+    (*| resF_Chk false _ => resF_Syn None*)
+    | _                => resF_Syn None
+    end ;                            (* error or annotation needed: *)
+bidirCheckF' g df dtv e0 SynF      := resF_Syn None.
+  Obligation 8.
+  pose proof Nat.le_max_l (edepth e) (edepth e');
+  left; apply Nat.lt_succ_r; apply H.
+  Defined.
+  Obligation 9.
+  pose proof Nat.le_max_l (edepth e) (edepth e');
+  left; apply Nat.lt_succ_r; apply H.
+  Defined.
+  Obligation 13. (* of 27 *)
+  pose proof Nat.le_max_l (edepth e_x) (edepth e');
+  left; apply Nat.lt_succ_r; apply H.
+  Defined.
+  Obligation 14.
+  pose proof Nat.le_max_r (edepth e_x) (edepth e');
+  left; apply Nat.lt_succ_r; apply H.
+  Defined.
+  Obligation 17.
+  pose proof Nat.le_max_l (edepth e0) (Nat.max (edepth e1) (edepth e2));
+  left; apply Nat.lt_succ_r; apply H.
+  Defined.
+  Obligation 18. 
+  pose proof Nat.le_max_l (edepth e1) (edepth e2);
+  pose proof Nat.le_max_r (edepth e0) (Nat.max (edepth e1) (edepth e2));
+  left; apply Nat.lt_succ_r; 
+  apply Nat.le_trans with (Init.Nat.max (edepth e1) (edepth e2));
+  assumption.
+  Defined.
+  Obligation 19.
+  pose proof Nat.le_max_r (edepth e1) (edepth e2);
+  pose proof Nat.le_max_r (edepth e0) (Nat.max (edepth e1) (edepth e2));
+  left; apply Nat.lt_succ_r; 
+  apply Nat.le_trans with (Init.Nat.max (edepth e1) (edepth e2));
+  assumption.
+  Defined.
+  Obligation 22.
+  pose proof Nat.le_max_l (edepth eH) (edepth eT);
+  left; apply Nat.lt_succ_r; apply H.
+  Defined.
+  Obligation 23.
+  pose proof Nat.le_max_r (edepth eH) (edepth eT);
+  left; apply Nat.lt_succ_r; apply H.
+  Defined.
+  Obligation 24.
+  pose proof Nat.le_max_l (edepth e) (Nat.max (edepth eN) (edepth eC));
+  left; apply Nat.lt_succ_r; apply H.
+  Defined.
+  Obligation 25.
+  pose proof Nat.le_max_l (edepth eN) (edepth eC);
+  pose proof Nat.le_max_r (edepth e) (Nat.max (edepth eN) (edepth eC));
+  left; apply Nat.lt_succ_r; 
+  apply Nat.le_trans with (Init.Nat.max (edepth eN) (edepth eC));
+  assumption.
+  Defined.
+  Obligation 26.
+  pose proof Nat.le_max_r (edepth eN) (edepth eC);
+  pose proof Nat.le_max_r (edepth e)  (Nat.max (edepth eN) (edepth eC));
+  left; apply Nat.lt_succ_r; 
+  apply Nat.le_trans with (Init.Nat.max (edepth eN) (edepth eC));
+  assumption.
+  Defined.
+
+
+Definition checkF' (g:fenv) (df:deBruijnsF) (dtv:deBruijnTVs) 
+                   (e:expr) (t:ftype) : bool :=
+    match bidirCheckF' g df dtv e (ChkF t) return bool with
+    | resF_Chk true  _t => ftype_eq t _t
+    | resF_Chk false _  => false 
+    (*| resF_Chk b _ => b*)
+    | _                 => false 
+    end.
+
+Definition synthF' (g:fenv) (df:deBruijnsF) (dtv:deBruijnTVs) 
+                  (e:expr) : option ftype :=
+    match bidirCheckF' g df dtv e SynF return (option ftype) with
+    | resF_Syn (Some t) => Some t 
+    | resF_Syn None     => None
+    | _CheckF           => None : option ftype
+    end.
+
+Definition checkF (g:fenv) (e:expr) (t:ftype) : bool := checkF' g DFEmpty DTEmpty e t.
+Definition synthF (g:fenv) (e:expr) : option ftype := synthF' g DFEmpty DTEmpty e.
+
+Inductive CheckF' : fenv -> deBruijnsF -> deBruijnTVs -> expr -> ftype -> Prop :=
+    | FChkLam   : forall (g:fenv) (df:deBruijnsF) (dtv:deBruijnTVs) (e':expr) (tx t':ftype),
+        isWFFT' g dtv tx Star -> CheckF' g (DFBind tx df) dtv e' t' 
+            -> CheckF' g df dtv (Lambda e') (FTFunc tx t')
+    | FChkLamT  :  forall (g:fenv) (df:deBruijnsF) (dtv:deBruijnTVs) 
+                          (k:kind) (e:expr) (t:ftype),
+        CheckF' g df (DTBind k dtv) e t -> CheckF' g df dtv (LambdaT k e) (FTPoly k t)
+    | FChkLet   : forall (g:fenv) (df:deBruijnsF) (dtv:deBruijnTVs) 
+                         (e_x e':expr) (t_x t':ftype),
+        SynthF' g df dtv e_x t_x -> CheckF' g (DFBind t_x df) dtv e' t'
+            -> CheckF' g df dtv (Let e_x e') t'
+    | FChkIf    : forall (g:fenv) (df:deBruijnsF) (dtv:deBruijnTVs) 
+                        (e0 e1 e2: expr) (t:ftype),
+        CheckF' g df dtv e0 (FTBasic TBool)
+            -> CheckF' g df dtv e1 t -> CheckF' g df dtv e2 t
+            -> CheckF' g df dtv (If e0 e1 e2) t            
+    | FChkSwit :  forall (g:fenv) (df:deBruijnsF) (dtv:deBruijnTVs) (e eN eC:expr) (t t':ftype),
+        SynthF' g df dtv e (FTList t) -> CheckF' g df dtv eN t'
+            -> CheckF' g df dtv eC (FTFunc t (FTFunc (FTList t) t'))
+            -> CheckF' g df dtv (Switch e eN eC) t'
+    | FChkSyn   : forall (g:fenv) (df:deBruijnsF) (dtv:deBruijnTVs) (e:expr) (t:ftype),
+        SynthF' g df dtv e t -> CheckF' g df dtv e t 
+
+with SynthF' : fenv -> deBruijnsF -> deBruijnTVs -> expr -> ftype -> Prop :=
+    | FSynBC    : forall (g:fenv) (df:deBruijnsF) (dtv:deBruijnTVs) (b:bool), 
+        SynthF' g df dtv (Bc b) (FTBasic TBool)
+    | FSynIC    : forall (g:fenv) (df:deBruijnsF) (dtv:deBruijnTVs) (n:Z),
+        SynthF' g df dtv (Ic n) (FTBasic TInt)
+    | FSynPrm   : forall (g:fenv) (df:deBruijnsF) (dtv:deBruijnTVs) (c:prim),
+        SynthF' g df dtv (Prim c) (erase_ty c) 
+    | FSynBV    : forall (g:fenv) (df:deBruijnsF) (dtv:deBruijnTVs) (i:index) (t:ftype),
+        bv_bound_inF i t df -> SynthF' g df dtv (BV i) t
+    | FSynFV    : forall (g:fenv) (df:deBruijnsF) (dtv:deBruijnTVs) (x:vname) (t:ftype),
+        bound_inF x t g -> SynthF' g df dtv (FV x) t
+    | FSynApp   : forall (g:fenv) (df:deBruijnsF) (dtv:deBruijnTVs)
+                         (e e':expr) (t_x t:ftype),
+        SynthF' g df dtv e (FTFunc t_x t) -> CheckF' g df dtv e t_x
+            -> SynthF' g df dtv (App e e') t
+    | FSynAppT  : forall (g:fenv) (df:deBruijnsF) (dtv:deBruijnTVs) 
+                         (e:expr) (k:kind) (s:ftype) (rt:type),
+        isMono rt -> noExists rt -> isLCT_at (dflen df) (dtlen dtv) rt 
+            -> Subset (free rt) (vbindsF g) -> Subset (freeTV rt) (tvbindsF g)
+            -> isWFFT' g dtv (erase rt) Star
+            -> SynthF' g df dtv e (FTPoly k s)
+            -> SynthF' g df dtv (AppT e rt) (ftsubBV (erase rt) s)      
+    | FSynAnn   : forall (g:fenv) (df:deBruijnsF) (dtv:deBruijnTVs) (e:expr) (rt:type),
+        isLCT_at (dflen df) (dtlen dtv) rt 
+            -> Subset (free rt) (vbindsF g) -> Subset (freeTV rt) (tvbindsF g)
+            -> CheckF' g df dtv e (erase rt) -> SynthF' g df dtv (Annot e rt) (erase rt)   
+    | FChkNil   : forall (g:fenv) (df:deBruijnsF) (dtv:deBruijnTVs) (t:type),
+        isWFFT' g dtv (erase t) Star -> SynthF' g df dtv (Nil t) (FTList (erase t))
+    | FSynCons  : forall (g:fenv) (df:deBruijnsF) (dtv:deBruijnTVs) (eH eT:expr) (t:type),
+        CheckF' g df dtv eH (erase t) -> CheckF' g df dtv eT (FTList (erase t))
+            -> SynthF' g df dtv (Cons t eH eT) (FTList (erase t)).
+
+Scheme CheckF_mutind  := Induction for CheckF'  Sort Prop
+with   SynthF_mutind  := Induction for SynthF'  Sort Prop.
+Combined Scheme BidirF_mutind from CheckF_mutind, SynthF_mutind.    
+
+Definition CheckF (g:fenv) (e:expr) (t:ftype) : Prop := 
+  CheckF' g DFEmpty DTEmpty e t.
+
+Definition SynthF (g:fenv) (e:expr) (t:ftype) : Prop := 
+  SynthF' g DFEmpty DTEmpty e t.
+
+(* From the bidirectional algorithm to the declaritive bidirectional typing *)
+Lemma lem_bidirCheckF'_CheckF'_helper : 
+  forall (n:nat) (g:fenv) (df:deBruijnsF) (dtv:deBruijnTVs)         
+         (e:expr) (t:ftype),
+    (2 * edepth e + 1 <= n
+        -> bidirCheckF' g df dtv e (ChkF t) = resF_Chk true t 
+        -> CheckF' g df dtv e t) /\ 
+    (2 * edepth e <= n
+        -> bidirCheckF' g df dtv e SynF = resF_Syn (Some t) 
+        -> SynthF' g df dtv e t).
+Proof. intros n; induction n.
+  - (* Base: n = 0 *) intros; split; intros;
+    (assert (2 * edepth e + 1 = 0)  by auto with *) ||
+    (assert (2 * edepth e = 0)      by auto with *);
+    repeat (apply Nat.eq_add_0 in H1; destruct H1);
+    try discriminate (* Chk mode is impossible *).
+    destruct e;   simpl in H1; try discriminate H1;
+    try rewrite bidirCheckF'_equation_2 in H0;
+    try rewrite bidirCheckF'_equation_4 in H0;
+    try rewrite bidirCheckF'_equation_6 in H0;
+    try rewrite bidirCheckF'_equation_8 in H0;
+    try rewrite bidirCheckF'_equation_10 in H0;
+    try rewrite bidirCheckF'_equation_26 in H0;
+    try rewrite bidirCheckF'_equation_32 in H0;
+    try destruct (isWFFT'_dec g dtv (erase t0) Star) eqn:Hwf;
+    try unfold isWFFTb' in H0; try rewrite Hwf in H0;
+    injection H0 as H0;
+    try subst t; try discriminate; try constructor;
+    try apply lem_lookupDF_bvboundinF;
+    try apply lem_lookupF_boundinF; trivial.
+  - (* Inductive: n > 0 *) intros; split; intros;
+    destruct e eqn:E;
+    (* avoid proving base case again *)
+    try ( assert (2 * edepth e <= n) as Hbase
+            by (rewrite E; simpl; auto with *);
+          apply IHn; subst e; assumption);
+    simpl in H; apply Nat.succ_le_mono in H;
+
+    try (
+      (
+        rewrite bidirCheckF'_equation_1 in H0;
+        destruct (bidirCheckF' g df dtv (Bc b) SynF) eqn:H'
+      ) || (
+        rewrite bidirCheckF'_equation_3 in H0;
+        destruct (bidirCheckF' g df dtv (Ic n0) SynF) eqn:H'
+      ) || (
+        rewrite bidirCheckF'_equation_5 in H0;
+        destruct (bidirCheckF' g df dtv (Prim p) SynF) eqn:H'
+      ) || (
+        rewrite bidirCheckF'_equation_7 in H0;
+        destruct (bidirCheckF' g df dtv (BV i) SynF) eqn:H'
+      ) || (
+        rewrite bidirCheckF'_equation_9 in H0;
+        destruct (bidirCheckF' g df dtv (FV x) SynF) eqn:H'
+      ) || (
+        rewrite bidirCheckF'_equation_13 in H0;
+        destruct (bidirCheckF' g df dtv (App e0_1 e0_2) SynF) eqn:H'
+      ) || (
+        rewrite bidirCheckF'_equation_17 in H0;
+        destruct (bidirCheckF' g df dtv (AppT e0 t0) SynF) eqn:H'
+      ) || (
+        rewrite bidirCheckF'_equation_21 in H0;
+        destruct (bidirCheckF' g df dtv (Annot e0 t0) SynF) eqn:H'
+      ) || (
+        rewrite bidirCheckF'_equation_25 in H0;
+        destruct (bidirCheckF' g df dtv (Nil t0) SynF) eqn:H'
+      ) || (
+        rewrite bidirCheckF'_equation_27 in H0;
+        destruct (bidirCheckF' g df dtv (Cons t0 e0_1 e0_2) SynF) eqn:H'
+      ) || (
+        rewrite bidirCheckF'_equation_31 in H0;
+        destruct (bidirCheckF' g df dtv Error SynF) eqn:H'
+      );
+      try destruct ot; try discriminate;
+      injection H0 as H0; 
+      apply lem_ftype_eq in H0; subst f;
+      apply FChkSyn; apply IHn; simpl; auto with *
+    ).
+  * (* FChkLam *) destruct t eqn:T;
+    rewrite bidirCheckF'_equation_11 in H0; try discriminate;
+    destruct (bidirCheckF' g (DFBind f1 df) dtv e0 (ChkF f2)) eqn:H';
+    try discriminate; injection H0 as H0.
+    apply Bool.andb_true_iff in H0; destruct H0;
+    apply Bool.andb_true_iff in H0; destruct H0; subst b.
+    apply FChkLam; try apply IHn; simpl;
+    try apply lem_isWFFTb_isWFFT'; apply lem_ftype_eq in H2;
+    subst t0; auto with * .   
+  * (* FChkLamT *) destruct t eqn:T;
+    rewrite bidirCheckF'_equation_15 in H0; try discriminate;
+    destruct (bidirCheckF' g df (DTBind k dtv) e0 (ChkF f)) eqn:H';
+    try discriminate; injection H0 as H0.
+    apply Bool.andb_true_iff in H0; destruct H0;
+    apply Bool.andb_true_iff in H0; destruct H0; subst b.
+    apply lem_kind_eq in H0; subst k0;
+    apply lem_ftype_eq in H2; subst f.
+    apply FChkLamT; apply IHn; auto with *.  
+  * (* FChkLet *) rewrite bidirCheckF'_equation_19 in H0;
+    destruct (bidirCheckF' g df dtv e0_1 SynF) eqn:H';
+    try destruct ot; try discriminate.
+    apply FChkLet with f; apply IHn; auto with *.
+  * (* FChkIf *) rewrite bidirCheckF'_equation_23 in H0;
+    destruct (bidirCheckF' g df dtv e0_1 (ChkF (FTBasic TBool))) eqn:H';
+    destruct (bidirCheckF' g df dtv e0_2 (ChkF t)) eqn:H'';
+    try destruct (bidirCheckF' g df dtv e0_3 (ChkF t1)) eqn:H''';
+    try discriminate; injection H0 as H0. 
+    apply Bool.andb_true_iff in H0; destruct H0;
+    apply Bool.andb_true_iff in H0; destruct H0; subst b b0 b1.
+    apply FChkIf; apply IHn; auto with *.
+(*      
+  * (* FChkSwit *)
+  * (* FSynBC  *)
+  * (* FSynIC  *)
+  * (* FSynPrm *)
+  * (* FSynBV  *)
+  * (* FSynFV  *)
+  * (* FSynApp  *)
+  * (* FSynAppT  *)
+  * (* FSynAnn  *)
+  * (* FChkNil  *)
+  * (* FSynCons  *)
+*)
+  Admitted.  
+
+Lemma lem_bidirCheckF'_CheckF' : 
+  forall (g:fenv) (df:deBruijnsF) (dtv:deBruijnTVs)         
+         (e:expr) (t:ftype),
+    bidirCheckF' g df dtv e (ChkF t) = resF_Chk true t 
+        -> CheckF' g df dtv e t.
+Proof. intros; 
+  apply lem_bidirCheckF'_CheckF'_helper with (2 * edepth e + 1);
+  trivial. Qed.
+
+Lemma lem_bidirCheckF'_SynthF' : 
+  forall (g:fenv) (df:deBruijnsF) (dtv:deBruijnTVs)         
+         (e:expr) (t:ftype),
+    bidirCheckF' g df dtv e SynF = resF_Syn (Some t) 
+        -> SynthF' g df dtv e t.
+Proof. intros; 
+  apply lem_bidirCheckF'_CheckF'_helper with (2 * edepth e);
+  trivial. Qed.
+
+Lemma lem_checkF'_CheckF' : 
+  forall (g:fenv) (df:deBruijnsF) (dtv:deBruijnTVs)         
+         (e:expr) (t:ftype),
+    checkF' g df dtv e t = true -> CheckF' g df dtv e t.
+Proof. intros. unfold checkF' in H. 
+  destruct (bidirCheckF' g df dtv e  (ChkF t)) eqn:H1;
+  try destruct b; try discriminate;
+  apply lem_ftype_eq in H; subst t0.
+  apply lem_bidirCheckF'_CheckF'; assumption. Qed.
+
+Lemma lem_synthF'_SynthF' : 
+  forall (g:fenv) (df:deBruijnsF) (dtv:deBruijnTVs)         
+         (e:expr) (t:ftype),
+    synthF' g df dtv e  = Some t -> SynthF' g df dtv e t.
+Proof. intros. unfold synthF' in H. 
+  destruct (bidirCheckF' g df dtv e  SynF) eqn:H1;
+  try destruct ot; try discriminate;
+  injection H as H; subst f.
+  apply lem_bidirCheckF'_SynthF'; assumption. Qed.
+         
+         (*
+Lemma lem_CheckF_open_tv_at : forall (g:fenv) (df:deBruijnsF) (dtv:deBruijnTVs) 
+                                     (e:expr) (t:ftype) (a:vname) (k:kind),
+    CheckF' g df (concatDT (DTBind k DTEmpty) dtv) e t
+        -> ~ in_envF a g 
+        -> CheckF' (FConsT a k g) df dtv (open_tv_at (dtlen dtv) a e) t.
+(* and SynthF *)
+    
+Lemma lem_CheckF_unbind_tv : forall (g:fenv) (e:expr) (t:ftype) (a:vname) (k:kind),
+    CheckF' g DFEmpty (DTBind k DTEmpty) e t -> ~ in_envF a g 
+        -> CheckF (FConsT a k g) (unbind_tv a e) t.
+(* and SynthF *)
+*)
+
+(* For next time: this isn't easy because we can't do structural
+    induction on CheckF'/SynthF' 
+    -- the IH will only apply to a subtree, which would be 
+        the check for e' w/ deBruijn envs when checking Lambda e'.
+    -- but we need is to apply IH to (unbind y e') for any
+        fresh enough y. 
+    => we need to do the tricky induction on edepth e + 0/1 again *)
+
+(* From declarative bidirectional typing to our typing judgment *)
+Lemma lem_CheckF_SynthF_HasFtype : (
+    forall (g:fenv) (df:deBruijnsF) (dtv:deBruijnTVs) (e:expr) (t:ftype),
+      CheckF' g df dtv e t -> df = DFEmpty 
+                           -> dtv = DTEmpty -> HasFtype g e t ) /\ (
+    forall (g:fenv) (df:deBruijnsF) (dtv:deBruijnTVs) (e:expr) (t:ftype),
+      SynthF' g df dtv e t -> df = DFEmpty 
+                           -> dtv = DTEmpty -> HasFtype g e t ) .
+Proof. apply ( BidirF_mutind
+    (fun (g:fenv) (df:deBruijnsF) (dtv:deBruijnTVs) 
+         (e:expr) (t:ftype) (chk_e_t : CheckF' g df dtv e t) => 
+        df = DFEmpty -> dtv = DTEmpty -> HasFtype g e t)
+    (fun (g:fenv) (df:deBruijnsF) (dtv:deBruijnTVs) 
+         (e:expr) (t:ftype) (syn_e_t : SynthF' g df dtv e t) =>
+        df = DFEmpty -> dtv = DTEmpty -> HasFtype g e t)
+  ); intros.
+  - apply FTAbs with Star (bindsF g).
+
+
+(* standalone CheckF? *)
+(* and SynthF *)
+
+
+(* use below maybe *)
+(* also a section of decidabili*)
+
+(*
+--        -> { a:Vname | not (in_envF a g) && not (Set_mem a (ffreeTV t)) } 
+--                                         && not (Set_mem a (ffreeTV t)) } 
+{-@ lem_checkType_unbindFT :: g:FEnv -> ae:AnonEnv -> i:Index -> k':Kind -> { e:Expr | noDefnsBaseAppT e }
+        -> { t:FType| checkType g (AConsT i k' ae) e t } 
+        -> { a:Vname | not (in_envF a g) && not (Set_mem a (fv e)) && not (Set_mem a (ftv e)) }
+        -> { pf:_ | checkType (FConsT a k' g) ae (open_tv_at i a e) (openFT_at i a t) } / [esize e] @-}
+lem_checkType_unbindFT :: FEnv -> AnonEnv -> Index -> Kind -> Expr -> FType  -> Vname -> Proof
+lem_checkType_unbindFT g ae i k' (Bc _) t a         = ()
+lem_checkType_unbindFT g ae i k' (Ic _) t a         = ()
+lem_checkType_unbindFT g ae i k' (Prim _ ) t a      = () -- rej
+lem_checkType_unbindFT g ae i k' (BV j) t a | j == i     = () -- rej, not relevant?
+                                            | otherwise  = () ? toProof ( bound_inAE j t (AConsT i k' ae) === bound_inAE j t ae )
+lem_checkType_unbindFT g ae i k' (FV x) t a | a == x     = () -- impossible!
+                                            | otherwise  = () ? toProof ( bound_inF x t (FConsT a k' g) === bound_inF x t g)
+lem_checkType_unbindFT g ae i k' (App e e') t a     = case ( synthType g (AConsT i k' ae) e' ) of
+    (Just t')       -> () ? lem_checkType_unbindFT g ae i k' e (FTFunc t' t) a
+                          ? lem_synthType_unbindFT g ae i k' e' t' a
+--    _               -> () -- ? lem_synthType_unbindFT g ae i k' e' t' a
+-- case ( synthType (FConsT a k' g) ae (open_tv_at i a e') ) of
+lem_checkType_unbindFT g ae i k' (AppT e t2) t a    = case ( synthType g (AConsT i k' ae) e ) of
+    (Just (FTPoly Base t1))  -> () ? lem_isWFFT_unbindFT    g ae i k' (erase t2) Base a
+                                   ? lem_synthType_unbindFT g ae i k' e (FTPoly Base t1) a
+--    _               -> impossible ("by lem" ? lem_synthType_unbindFT 
+lem_checkType_unbindFT g ae i k' (Annot e liqt) t a = () ? lem_checkType_unbindFT g ae i k' e t {-(erase liqt)-} a
+                                                         ? lem_erase_open_tvT_at i a liqt -- local cl?
+--                                       && not (Set_mem a (ffreeTV t)) } 
+{-@ lem_synthType_unbindFT :: g:FEnv -> ae:AnonEnv -> i:Index -> k':Kind -> { e:Expr | noDefnsBaseAppT e }
+      -> { t:FType | synthType g (AConsT i k' ae) e  == Just t } 
+      -> { a:Vname | not (in_envF a g) && not (Set_mem a (fv e)) && not (Set_mem a (ftv e)) }
+      -> { pf:_ | synthType (FConsT a k' g) ae (open_tv_at i a e) == Just (openFT_at i a t) } / [esize e] @-}
+lem_synthType_unbindFT :: FEnv -> AnonEnv -> Index -> Kind -> Expr -> FType  -> Vname -> Proof
+lem_synthType_unbindFT g ae i k' (Bc _) t a         = ()
+lem_synthType_unbindFT g ae i k' (Ic _) t a         = ()
+lem_synthType_unbindFT g ae i k' (Prim _ ) t a      = ()
+lem_synthType_unbindFT g ae i k' (BV j) t a         = () ? toProof (lookupAE j (AConsT i k' ae) === lookupAE j ae)
+lem_synthType_unbindFT g ae i k' (FV x) t a         = () ? toProof (lookupF x (FConsT a k' g) === lookupF x g)
+lem_synthType_unbindFT g ae i k' (App e e') t a     = case ( synthType g (AConsT i k' ae) e' ) of
+    (Just t')       -> () ? lem_checkType_unbindFT g ae i k' e (FTFunc t' t) a
+                          ? lem_synthType_unbindFT g ae i k' e' t' a 
+lem_synthType_unbindFT g ae i k' (AppT e t2) t a    = case ( synthType g (AConsT i k' ae) e ) of
+    (Just (FTPoly Base t1)) -> () ? lem_isWFFT_unbindFT    g ae i k' (erase t2) Base a
+                                  ? lem_synthType_unbindFT g ae i k' e (FTPoly Base t1) a
+lem_synthType_unbindFT g ae i k' (Annot e liqt) t a = () ? lem_checkType_unbindFT g ae i k' e t {-(erase liqt)-} a
+                                                         ? lem_erase_open_tvT_at i a liqt
+{-@ lem_check_synth :: g:FEnv -> { e:Expr | noDefnsBaseAppT e } 
+        -> { t:FType | synthType g AEmpty e == Just t } -> { pf:_ | checkType g AEmpty e t } @-}
+lem_check_synth :: FEnv -> Expr -> FType -> Proof
+lem_check_synth g (Bc b) t         = case t of 
+    (FTBasic TBool) -> ()
+lem_check_synth g (Ic n) t         = case t of
+    (FTBasic TInt)  -> () 
+lem_check_synth g (Prim c) t       = ()
+lem_check_synth g (FV x) t         = lem_lookup_boundinF x t g 
+lem_check_synth g (App e e') t     = case (synthType g AEmpty e') of
+    (Just t')       -> lem_check_synth g e (FTFunc t' t)   -- where  (Just t') = synthType g e' 
+    Nothing         -> impossible ""
+lem_check_synth g (AppT e t2) t    = case (synthType g AEmpty e) of 
+    (Just (FTPoly Base t1))  -> ()
+lem_check_synth g (Annot e liqt) t = ()
+
+{-@ makeHasFType :: g:FEnv -> { e:Expr | noDefnsBaseAppT e } -> { t:FType | checkType g AEmpty e t }
+        -> ProofOf(HasFType g e t) / [esize e] @-}
+makeHasFType :: FEnv -> Expr -> FType -> HasFType
+makeHasFType g (Bc b) t         = case t of
+    (FTBasic TBool) -> FTBC g b
+makeHasFType g (Ic n) t         = case t of
+    (FTBasic TInt)  -> FTIC g n
+makeHasFType g (Prim c) t       = FTPrm g c
+makeHasFType g (FV x) t         = simpleFTVar g (x? lem_boundin_inenvF x t g ) t
+makeHasFType g (App e e') t     = FTApp g e t' t pf_e_t't e' pf_e'_t'
+  where
+    (Just t')  = synthType g AEmpty e'
+    pf_e_t't   = makeHasFType g e (FTFunc t' t)
+    pf_e'_t'   = makeHasFType g e' (t' ? lem_check_synth g e' t')
+makeHasFType g (AppT e rt) t    = case (synthType g AEmpty e) of 
+  (Just (FTPoly Base t1)) -> FTAppT g e Base t1 pf_e_at1 rt pf_rt_wfft 
+    where
+      pf_e_at1        = makeHasFType g e (FTPoly Base t1 ? lem_check_synth g e (FTPoly Base t1)) 
+      pf_rt_wfft      = makeWFFT g (erase rt ? lem_erase_freeTV rt
+                                             ? toProof ( S.isSubsetOf (freeTV rt) (tvbindsF g) && 
+                                                         S.isSubsetOf (tvbindsF g) (bindsF g) )) Base 
+makeHasFType g (Annot e liqt) t = FTAnn g e t liqt pf_e_t
+  where
+    pf_e_t = makeHasFType g e t
+
+(* the only possible type a preds can have is FTBasic TBool *)
+Fixpoint checkP' (g:fenv) (df:deBruijnsF) (dtv:deBruijnTVs) (ps:preds) : Prop :=
+    match ps with 
+    | PEmpty      => True
+    | PCons q qs  => CheckF' g df dtv q (FTBasic TBool) /\ checkP' g df dtv qs
+    end.
+
+Definition checkP (g:fenv) (ps:preds) : Prop := checkP' g DFEmpty DTEmpty ps.
+
+
+{-@ makePHasFType :: g:FEnv -> { ps:Preds | allNoDefnsBaseAppT ps && checkPreds g AEmpty ps } 
+       	-> ProofOf(PHasFType g ps) / [predsize ps] @-}
+makePHasFType :: FEnv -> Preds -> PHasFType 
+makePHasFType g PEmpty       = PFTEmp  g
+makePHasFType g (PCons p ps) = PFTCons g p (makeHasFType g p (FTBasic TBool))
+                                       ps (makePHasFType g ps)
+
+Lemma lem_isWFFT_openFT_at : 
+  forall (g:fenv) (t:ftype) (k:kind) (k':kind) (d:deBruijnTVs) (a:vname),
+           isWFFT' g (concatDT (DTBind k' DTEmpty) d) t k
+        -> ~ in_envF a g 
+        -> isWFFT' (FConsT a k' g) d (openFT_at (dtlen d) a t) k.
+Proof. intros g; induction t.
+  - (* FTBasic *) intros. destruct b; simpl in H; simpl; try apply I.
+    * (* BTV *) 
+      destruct H; simpl in H; try destruct H;
+      apply lem_btvboundin_append in H; destruct H; destruct H;
+      try assert (dtlen d =? i = true)
+         by (apply Nat.eqb_eq; symmetry; apply H);
+      try assert (dtlen d =? i = false)
+         by (apply Nat.eqb_neq; auto with *); 
+      rewrite H3 || rewrite H2; simpl; intuition.
+    * (* FTV *) destruct H; [left|right]; try destruct H;
+      try split; try right; trivial.
+  - (* FTFunc *) intros; simpl; simpl in H; destruct H; destruct H1;
+    split; try split; try apply IHt1; try apply IHt2; trivial.
+  - (* FTPoly *) intros; simpl; simpl in H; destruct H; split;
+    try apply IHt; trivial.
+  - (* FTList *) intros; simpl; simpl in H; destruct H; split;
+    try apply IHt; trivial.
+  Qed.
+
+Lemma lem_isWFFT_unbindFT : 
+  forall (g:fenv) (t:ftype) (k:kind) (k':kind) (a:vname),
+           isWFFT' g (DTBind k' DTEmpty) t k-> ~ in_envF a g 
+        -> isWFFT (FConsT a k' g) (unbindFT a t) k.
+Proof. intros; apply lem_isWFFT_openFT_at; simpl; trivial. Qed.
+
+
+Lemma makeWFFT' : forall (n:nat) (g:fenv) (t:ftype) (k:kind),
+    fdepth t <= n   -> isWFFT g t k -> WFFT g t k.
+Proof. intros n; induction n.
+  - (* Base *) intros;
+    assert (fdepth t = 0) by auto with *.
+    destruct t; simpl in H1; try discriminate.
+    destruct b; unfold isWFFT in H0; simpl in H0;
+    destruct k; try destruct H0;
+    try destruct H0; try discriminate;
+    try (destruct i; contradiction);
+    try (apply WFFTFV; apply H0);
+    try apply WFFTKind; try apply WFFTFV; 
+    try apply WFFTBasic; simpl; trivial.
+  - (* Inductive *) intros.
+    destruct t eqn:T;
+    (* avoid proving base case again *)
+    try (assert (fdepth t <= n) as Hbase
+          by (rewrite T; simpl; auto with *);
+         apply IHn; subst t; trivial);
+    simpl in H; apply Nat.succ_le_mono in H.
+    * (* FTFunc t1 t2 *)
+      unfold isWFFT in H0; 
+      destruct H0; destruct H1; subst k.
+      apply WFFTFunc with Star Star; 
+      apply IHn; try apply Nat.le_trans 
+        with (Init.Nat.max (fdepth f1) (fdepth f2));
+      try apply Nat.le_max_l;
+      try apply Nat.le_max_r; trivial.
+    * (* FTPoly k0 f *)
+      unfold isWFFT in H0; destruct H0; subst k.
+      apply WFFTPoly with Star (bindsF g);
+      intros; apply IHn; try rewrite fdepth_unbindFT;
+      try apply lem_isWFFT_unbindFT; trivial.
+    * (* FTList f *) 
+      unfold isWFFT in H0; destruct H0; subst k.
+      apply WFFTList with Star; apply IHn; trivial.
+  Qed.
+
+Theorem makeWFFT : forall (g:fenv) (t:ftype) (k:kind),
+    isWFFT g t k -> WFFT g t k.
+Proof. intros. apply makeWFFT' with (fdepth t); trivial. Qed.
