coq-SystemRF-3.1/Bidirectional/SynthTyping.v
@@ -1,0 +1,435 @@
+Require Import SystemRF.BasicDefinitions. 
+Require Import SystemRF.Names.
+Require Import SystemRF.BasicPropsEnvironments.
+Require Import SystemRF.SystemFWellFormedness.
+Require Import SystemRF.SystemFTyping.
+Require Import Bidirectional.Decidable.
+Require Import Bidirectional.SynthWFFT.
+Require Import Bidirectional.SynthFType.
+Require Import Bidirectional.SynthWFtype.
+
+From Equations Require Import Equations.
+
+Require Import Arith.
+Require Import ZArith.
+Require Import Lists.ListSet.
+
+Fixpoint lookup (x : vname) (g : env) : option type :=
+    match g with 
+    | Empty           => None
+    | ECons x' t' g'  => if (x =? x') then Some t' else lookup x g'
+    | EConsT a' k' g' => lookup x g'
+    end.
+
+(*----------------------------------------------------------------------------
+  --- | ABSTRACT MODEL of VERIFICATION CONDITIONS
+  --------------------------------------------------------------------------*)
+
+Inductive sort : Set :=
+    | Bool
+    | Int
+    | BTVar (i : index)
+    | FTVar (a : vname)
+    | List                  (* s : sort ? *)
+    | Ignore.
+
+Definition toSort (b : basic) : sort :=
+    match b with 
+    | TBool     => Bool
+    | TInt      => Int
+    | (BTV i)   => BTVar i
+    | (FTV a)   => FTVar a
+    end.
+
+Inductive VC : Set :=
+    | Pred (ps : preds)
+    | Conj (c : VC) (c' : VC)
+    | ForAll (b:sort) (ps:preds) (c : VC) (* nameless binder *)
+    | ForAllFV (x:vname) (b:sort) (ps:preds) (c:VC).
+        (* if we start w/ an Empty env then this case never occurs *)
+
+Definition trueC : VC := Pred PEmpty.
+
+Definition mkVC (t_x : type) (c : VC) : VC :=
+    match t_x with
+    | (TRefn b ps) => ForAll (toSort b) ps c
+    | (TList t ps) => ForAll List       ps c
+    | _            => ForAll Ignore PEmpty c
+    end.
+
+Definition mkVCFV (x : vname) (t_x : type) (c : VC) : VC :=
+    match t_x with
+    | (TRefn b ps) => ForAllFV x (toSort b) ps c
+    | (TList t ps) => ForAllFV x List       ps c
+    | _            => ForAllFV x Ignore PEmpty c
+    end.
+
+(*----------------------------------------------------------------------------
+  --- | MODELLING VC/CONSTRAINTS AS COQ PROPS
+  --------------------------------------------------------------------------*)
+
+(* Draft solver: currently does not generate Props for polymoprhic VCs *)
+
+Definition sortToCoqType (s : sort) : Type :=
+    match s with
+    | Bool      => Some bool
+    | Int       => Some Z
+    | BTVar i   => None (* TODO *)
+    | FTVar a   => None (* TODO *)
+    | List      => Some (list unit)
+    | Ignore    => Some unit 
+    end.
+
+(*Fixpoint primToSetFn (p : prim) : 
+
+Fixpoint exprToSet   (ss : sorts) ()*)
+
+Fixpoint exprToProp (e : expr) : Prop := True. (* TODO *)
+
+Fixpoint predsToProp (ss : sorts) (ps : preds) : Prop :=
+    match ps with
+    | PEmpty      => True
+    | PCons p ps' => exprToProp p /\ predsToProp ps'
+    end.
+
+Fixpoint SMTtoProp' (*ss : sorts*) (c : VC) : Prop :=
+    match c with
+    | Pred ps             => predsToProp ps
+    | Conj c c'           => SMTtoProp c /\ SMTtoProp c'
+    | ForAll     b ps c   =>
+        match sortToCoqType s with 
+        | Some T => False (* TODO *)
+        | None   => False
+        end
+    | ForAllFV x b ps c   => 
+        match sortToCoqType s with 
+        | Some T => forall (x:T), predsToProp ps -> SMTtoProp c
+        | None   => False
+        end
+    end.
+
+Definition SMTtoProp (c : VC) : Prop := SMTtoProp' (* *) c. 
+
+(*----------------------------------------------------------------------------
+  --- | AUTOMATED INFERENCE of SYSTEM RF TYPING JUDGMENTS
+  --------------------------------------------------------------------------*)
+
+(* SUBTYPING: Note that UNLIKE the metatheory, the Check/Syn0th definition
+      is NOT mutually recursive with IsSub because existential types only
+      every appear on the LHS of obligations to check and therefore we never
+      have to guess or check a witness in S-Witn. *)
+
+(* option is used because we can reject some obligations out of hand *)
+
+Fixpoint isSubtype' (g:env) (dv:deBruijns) (dtv:deBruijnTVs) (t t':type) : option VC :=
+    match t, t' with 
+    | (TRefn b ps, TRefn b' qs)    
+          => if basic_eq b b'
+             then Some (ForAll (toSort b) ps (Pred qs))
+             else None
+    | (TFunc s_x s', TFunc t_x t')  
+          => match isSubtype' g dv dtv t_x s_x with
+             | Some c_x 
+                =>  match isSubtype' g (DVBind t_x dv) dtv s' t' with
+                    | Some c  => Conj c_x (mkVC t_x c)
+                    | None    => None
+                    end
+             | None => None
+             end
+    | (TExists s_x s, _) 
+          => match isSubtype' g (DVBind s_x dv) dtv s (shiftT t') with
+             | Some c => mkVC s_x c
+             | None   => None
+            end
+    | (TPoly k s, TPoly k' s')   
+          => if kind_eq k k'  (* we don't need to keep the kind info *)
+             then isSubtype' g dv (DTBind k dtv) s s' (* so return c as-is*)
+             else None
+    | (TList s ps, TList s' qs)   
+          => match isSubtype' g dv dtv s s' with
+             | Some c => Conj (c (ForAll List ps (Pred qs)))
+             | None   => None
+             end
+    end.      
+
+
+(* here is where we might plug in our various models of constraint solvers *)
+Inductive SMTValid : VC -> Prop :=
+    (* dummy solver *)
+    | SMTVtrivial  : SMTValid (Pred PEmpty)
+    | SMTVquant    : forall (b:sort) (ps:preds) (c:VC),
+        SMTValid c -> SMTValid (ForAll b ps c)
+    | SMTVconj     : forall (c c' : VC), 
+        SMTValid c -> SMTValid c' -> SMTValid (Conj c c')
+    (* prove constraints in Coq *)
+    | SMTVcoq      : forall (c:VC),
+        SMTtoProp c -> SMTValid c.
+
+Inductive Entails' : env -> deBruijns -> deBruijnTVs -> VC -> Prop :=
+    | EntEmp    : forall (c:VC),
+        SMTValid c -> Entails' Empty DVEmpty DTEmpty c
+    | EntExtFV  : forall (g:env) (dv:deBruijns) (dtv:deBruijnTVs) (x:vname) (tx:type) (c:VC),
+        Entails' g dv dtv (mkVCFV x tx c)  -> Entails' (ECons x tx g) dv dtv c
+    | EntExtBV  : forall (g:env) (dv:deBruijns) (dtv:deBruijnTVs) (tx:type) (c:VC),
+        Entails' g dv dtv (mkVC tx c)  -> Entails' g (DVBind tx dv) dtv c
+    | EntExtBTV : forall (g:env) (dv:deBruijns) (dtv:deBruijnTVs) (k:kind) (c:VC),
+        Entails' g dc dtv c -> Entails' g dv (DTBind k dtv) c.
+
+Definition Entails (c:VC) : Prop := Entails' Empty DVEmpty DTEmpty c.
+
+Inductive IsSubtype': env -> deBruijns -> deBruijnTVs -> type -> type -> Prop :=
+    | SubRefn : forall (g:env) (dv:deBruijns) (dtv:deBruijnTVs) (b:basic) (ps qs:preds),
+        Entails' g dv dtv (ForAll (toSort b) ps (Pred qs)) 
+            -> IsSubtype' g dv dtv (TRefn b ps) (TRefn b qs)
+    | SubFunc : forall (g:env) (dv:deBruijns) (dtv:deBruijnTVs) (s_x s' t_x t': type),
+        IsSubtype' g dv dtv t_x s_x -> IsSubtype' g (DVBind t_x dv) dtv s' t' 
+            -> IsSubtype' g dv dtv (TFunc s_x s') (TFunc t_x t')
+    | SubExis : forall (g:env) (dv:deBruijns) (dtv:deBruijnTVs) (s_x s t:type),
+        IsSubtype' g (DVBind s_x dv) dtv s (shiftT t') 
+            -> IsSubtype' g dv dtv (TExists s_x s) t
+    | SubPoly : forall (g:env) (dv:deBruijns) (dtv:deBruijnTVs) (k:kind) (s t:type),
+        IsSubtype' g dv (DTBind k dtv) s t
+            -> IsSubtype' g dv dtv (TPoly k s) (TPoly k t)
+    | SubList : forall (g:env) (dv:deBruijns) (dtv:deBruijnTVs) (s t:type) (ps qs:preds),
+        IsSubtype' g dv dtv s t
+            -> Entails' g dv dtv (ForAll List ps (Pred qs))
+            -> IsSubtype' g dv dtv (TList s ps) (TList t qs).
+
+(* TYPING *)
+(* one version is computable function, the other is a mutually inductive
+      prop that we prove is decidable using the first way *)
+
+Fixpoint check' (g:env) (dv:deBruijns) (dtv:deBruijnTVs) 
+                (e:expr) (t:type) : option VC := 
+    match e with          
+    | (Lambda e')     => 
+        match t with
+        | (TFunc t_x t')  => 
+            match isWFtypeb' g dv dtv t_x Star with
+            | true  =>
+                match check' g (DVBind t_x dv) dtv e' t' with
+                | Some c  => Some (mkVC t_x c)
+                | None    => None
+                end
+            | false => None
+            end
+        | _               => None 
+        end
+    | (LambdaT k e')  =>
+        match t with
+        | (TPoly k' t')   => 
+            match kind_eq k k' with
+            | true  => check' g dv (DTBind k dtv) e' t'
+            | False => None
+            end
+        | _               => None
+        end
+    | (Let e_x e')    =>
+        match isWFtypeb' g dv dtv t Star with
+        | true  =>
+            match synth' g dv dtv e_x with
+            | Some ( c1, t_x )  =>
+                match check' g (DVBind t_x dv) dtv e' t' with
+                | Some c2 => Some (Conj c1 (mkVC t_x c2))
+                | None    => None
+                end
+            | None              => None
+            end
+        | false => None
+        end
+    | (If e0 e1 e2)   => 
+        match isWFtypeb' g dv dtv t Star with
+        | true  => 
+            match check' g dv dtv e0 (TRefn TBool PEmpty) with
+            | Some c0 =>
+                match check' g (DVBind (self (TRefn TBool PEmpty) (Bc true) Base) dv) 
+                             dtv e1 (shiftT t) with
+                | Some c1 =>
+                    match check' g (DVBind (self (TRefn TBool PEmpty) (Bc false) Base) dv) 
+                          dtv e2 (shiftT t) with
+                    | Some c2 => Some (Conj c0 
+                                        (Conj (mkVC (self (TRefn TBool PEmpty) (Bc true) Base) c1) 
+                                           (mkVC (self (TRefn TBool PEmpty) (Bc false) Base) c2)))
+                    | None    => None
+                    end
+                | None    => None
+                end
+            | None    => None
+            end
+        | false => None
+        end
+    | Nil             =>
+        match t with 
+        | (TList t' ps) =>
+            match isMonob t' && noExistsb t' with
+            | true  =>
+                match isWFtypeb' g dv dtv (TList t' ps) Star with
+                | true  => isSubtype' g dv dtv (TPoly k s) (TList t' ps)
+                | false => None
+                end
+            | false => None
+            end
+        | _                 => None
+        end
+    | (Switch e eN eC) =>
+        match isWFtypeb' g dv dtv t Star with
+        | true  => 
+            match synth' g dv dtv e with
+            | Some (c, TList s ps)  =>
+                match check' g (DVBind (TList s (PCons (eq (Ic 0) (length s (BV 0))) ps)) dv) 
+                             dtv eN t with
+                | Some cN =>
+                    match check' g (DVBind (TList s (PCons (eq (App (Prim Succ) (length s (BV 1))) 
+                                                    (length s (BV 0))) ps))
+                                      (DVBind (TList s PEmpty) dv)) dtv eC
+                            (TFunc s (TFunc (TList s (PCons (eq (length s (BV 2)) 
+                                                          (length s (BV 0))) PEmpty)) t)) with
+                    | Some cC => Some (Conj c (Conj (mkVC (TList s (PCons (eq (Ic 0) (length s (BV 0))) ps)) cN) 
+                                                    (mkVC (TList s (PCons (eq (App (Prim Succ) (length s (BV 1))) 
+                                                                              (length s (BV 0))) ps)) 
+                                                          (mkVC (TList s PEmpty) cC))))
+                    | None    => None
+                    end
+                | None    => None
+                end
+            | _                     => None
+            end
+        | false => None
+        end
+    | _               => 
+        match (synth' g dv dtv e) with
+        | Some (c, s) => 
+            match isSubtype' g dv dtv s t with
+            | Some c'   => Some (Conj c c')
+            | None      => None
+            end
+        | None        => None
+        end
+    end
+
+with synth' (g:env) (dv:deBruijns) (dtv:deBruijnTVs) 
+            (e:expr) : option (VC * type) :=
+    match e with
+    | (Bc b)                => Some ( trueC, tybc b )
+    | (Ic n)                => Some ( trueC, tyic n )
+    | (Prim c)              => Some ( trueC, ty c )
+    | (BV i)                => 
+        match (lookupD i dv) with
+        | Some t  => Some ( trueC, self t (BV i) Base )
+        | None    => None
+        end
+    | (FV x)                => 
+        match (lookup x g) with
+        | Some t  => Some ( trueC, self t (FV x) Base )
+        | None    => None
+        end
+    | (App e e')            => 
+        match ( synth' g dv dtv e ) with
+        | (Some (c, TFunc t_x t)) =>
+            match ( check' g dv dtv e' t_x ) with
+            | Some c'  => Some ( Conj c c', TExists t_x t )
+            | _        => None
+            end
+        | _                     => None
+        end
+    | (AppT e' t)           =>
+        match isMonob t && noExistsb t with
+        | true  =>
+            match isWFtypeb' g dv dtv t Star with
+            | true  => 
+                match synth' g dv dtv e with
+                | Some (c, TPoly k s) => Some (c, tsubBTV t s)
+                | _                   => None
+                end
+            | false => None
+            end
+        | false => None
+        end
+    | (Annot e' t)          =>
+        match noExistsb t with
+        | true  =>
+            match ( check' g dv dtv e' t ) with
+            | Some c  => Some ( c, t )
+            | None    => None
+            end
+        | false => None
+        end
+    | Nil                   => 
+        match c (* TODO *)
+    | SynNil   : forall (g:env) (dv:deBruijns) (dtv:deBruijnTVs) (t : type),
+        Check' g dv dtv Nil (TList t PEmpty)
+            -> Synth' g dv dtv Nil (TList t (PCons (eq (Ic 0) (length t (BV 0))) PEmpty))    
+    | SynCons  : forall (g:env) (dv:deBruijns) (dtv:deBruijnTVs) (eH eT:expr) (t:type),
+        isMono t -> noExists t -> Synth' g dv dtv eT (TList t ps)
+            -> Check' g dv dtv eH t 
+            -> Synth' g dv dtv (Cons eH eT)
+                (TExists (TList t ps) (TList t 
+                  (PCons (eq (App (Prim Succ) (length t (BV 1))) (length t (BV 0))) PEmpty)))   
+    | _                     => None (* Error or annotation is needed *)
+    end.  
+    (* isWFtypeb' g dv dtv t Star  *)
+
+Inductive Check' : env -> deBruijns -> deBruijnTVs -> expr -> type -> Prop := 
+    | ChkLam   : forall (g:env) (dv:deBruijns) (dtv:deBruijnTVs) (e':expr) (tx t':type),
+        isWFtype' g dv dtv tx Star -> Check' g (DVBind tx dv) dtv e' t' 
+            -> Check' g dv dtv (Lambda e') (TFunc tx t')
+    | ChkLamT  :  forall (g:env) (dv:deBruijns) (dtv:deBruijnTVs) (k:kind) (e:expr) (t:type),
+        Check' g dv (DTBind k dtv) e t -> Check' g dv dtv (LambdaT k e) (TPoly k t)
+    | ChkLet   : forall (g:env) (dv:deBruijns) (dtv:deBruijnTVs) 
+                        (e_x e':expr) (tx t':type),
+        isWFtype' g dv dtv t Star -> Synth' g dv dtv e_x t_x
+            -> Check' g (DVBind t_x dv) dtv e' t'
+            -> Check' g dv dtv (Let e_x e') t'
+    | ChkIf    : forall (g:env) (dv:deBruijns) (dtv:deBruijnTVs) 
+                        (e0 e1 e2: expr) (t:type),
+        isWFtype' g dv dtv t Star -> Check' g dv dtv e0 (TRefn TBool PEmpty)
+            -> Check' g (DVBind (self (TRefn TBool PEmpty) (Bc true)  Base) dv) dtv e1 (shiftT t)
+            -> Check' g (DVBind (self (TRefn TBool PEmpty) (Bc false) Base) dv) dtv e2 (shiftT t)
+            -> Check' g dv dtv (If e0 e1 e2) t
+    | ChkNil   : forall (g:env) (dv:deBruijns) (dtv:deBruijnTVs) (t:type),
+        isMono t -> noExists t -> isWFtype' g dv dtv t Star 
+            -> Check' g dv dtv Nil (TList t PEmpty)
+    | ChkSwit :  forall (g:env) (dv:deBruijns) (dtv:deBruijnTVs) (e eN eC:expr) (t':type),
+        isWFtype' g dv dtv t' Star -> Synth' g dv dtv e (TList t ps)
+            -> Check' g (DVBind (TList t (PCons (eq (Ic 0) (length t (BV 0))) ps)) dv) dtv eN t'
+            -> Check' g (DVBind (TList t (PCons (eq (App (Prim Succ) (length t (BV 1))) 
+                                                    (length t (BV 0))) ps))
+                          (DVBind (TList t PEmpty) dv)) dtv eC
+                      (TFunc t (TFunc (TList t (PCons (eq (length t (BV 2)) 
+                                                          (length t (BV 0))) PEmpty)) t'))
+            -> Check' g dv dtv (Switch e eN eC) t'
+    | ChkSyn   : forall (g:env) (dv:deBruijns) (dtv:deBruijnTVs) (e:expr) (s t:type),
+        Synth' g dv dtv e s -> IsSubtype' g dv dtv s t 
+            -> Check' g dv dtv e t 
+
+with Synth' : env -> deBruijns -> deBruijnTVs -> expr -> type -> Prop := 
+    | SynBC    : forall (g:env) (dv:deBruijns) (dtv:deBruijnTVs) (b:bool), 
+        Synth' g dv dtv (Bc b) (tybc b)
+    | SynIC    : forall (g:env) (dv:deBruijns) (dtv:deBruijnTVs) (n:Z),
+        Synth' g dv dtv (Ic n) (tyic n)
+    | SynPrm   : forall (g:env) (dv:deBruijns) (dtv:deBruijnTVs) (c:prim),
+        Synth' g dv dtv (Prim c) (ty c) 
+    | SynBV    : forall (g:env) (df:deBruijns) (dtv:deBruijnTVs) (i:index) (t:type),
+        bv_bound_in i t dv -> Synth' g dv dtv (BV i) (self t (BV i) Base)
+    | SynFV    : forall (g:env) (dv:deBruijns) (dtv:deBruijnTVs) (x:vname) (t:type),
+        bound_in x t g -> Synth' g dv dtv (FV x) (self t (FV x) Base) 
+    | SynApp   : forall (g:env) (dv:deBruijns) (dtv:deBruijnTVs) 
+                        (e e':expr) (t_x t:type),
+        Synth' g dv dtv e (TFunc t_x t) -> Check' g dv dtv e t_x
+            -> Synth' g dv dtv (App e e') (TExists t_x t)
+    | SynAppT  : forall (g:env) (dv:deBruijns) (dtv:deBruijnTVs) 
+                        (e:expr) (k:kind) (s t:type),
+        isMono t -> noExists t -> isWFtype' g dv dtv t Star
+            -> Synth' g dv dtv e (TPoly k s)
+            -> Synth' g dv dtv (AppT e t) (tsubBTV t s)
+    | SynAnn   : forall (g:env) (dv:deBruijns) (dtv:deBruijnTVs) (e:expr) (t:type),
+        noExists t -> Check' g dv dtv e t -> Synth' g dv dtv (Annot e t) t 
+    | SynNil   : forall (g:env) (dv:deBruijns) (dtv:deBruijnTVs) (t : type),
+        Check' g dv dtv Nil (TList t PEmpty)
+            -> Synth' g dv dtv Nil (TList t (PCons (eq (Ic 0) (length t (BV 0))) PEmpty))    
+    | SynCons  : forall (g:env) (dv:deBruijns) (dtv:deBruijnTVs) (eH eT:expr) (t:type),
+        isMono t -> noExists t -> Synth' g dv dtv eT (TList t ps)
+            -> Check' g dv dtv eH t 
+            -> Synth' g dv dtv (Cons eH eT)
+                (TExists (TList t ps) (TList t 
+                  (PCons (eq (App (Prim Succ) (length t (BV 1))) (length t (BV 0))) PEmpty))).   
