coq-SystemRF-3.1/Bidirectional/Meeting0621.md
@@ -1,0 +1,36 @@
+me:
+check(gamma, e, t) : Prop
+synth(gamma, e) : option Type
+
+
+Today
+
+Ranjit Jhala  to  Everyone 3:45 PM
+Check(Gamma, e, t) => C
+Forall G, e, t . Let C = Check(Gamma, e, t). IF Valid(C) THEN G |- e : t
+
+Ranjit Jhala  to  Everyone 3:46 PM (Edited)
+`G |- e : t`   [POPL]
+
+G |- e << t   [NEW]
+G |- e >> t   [NEW]
+
+You  to  Everyone 3:47 PM
+forall .... : G |- e << t then G |- e : t
+
+Ranjit Jhala  to  Everyone 3:47 PM (Edited)
+* FORALL G,e,t. IF G |- e << t  THEN G |- e : t
+* FORALL G,e,t. IF G |- e >> t  THEN G |- e : t
+
+Ranjit Jhala  to  Everyone 3:49 PM
+* Forall G, e, t . Let C = Check(Gamma, e, t). IF Valid(C) THEN G |- e << t
+CHECK(Gamma, e, t) ==> Option(G |- e << t)
+ORACLE :: Gamma => P => Q => Bool
+Gamma |- P => Q
+
+Ranjit Jhala  to  Everyone 3:54 PM
+```
+type Oracle = g:Gamma -> p:Expr -> q:Expr -> Option ( g |- p => q )
+```
+Check :: Oracle -> g:Gamma -> e: Expr -> t: Type -> Option ( g |- e << t )
+Synth :: Oracle -> g:Gamma -> e: Expr -> Option (exists t. g |- e >> t )
