coq-SystemRF-3.1/compile_new.sh
@@ -1,0 +1,20 @@
+echo "Checking the SystemRF Mechanization"
+echo "-----------------------------------------------"
+echo "Version 3.0: Full 2023 RF proof + Lists"
+echo "-----------------------------------------------"
+
+echo "Up next: Implement the Bidirectional Typechecker / Proof Synthesizer"
+echo "Checking Decidable.v ..."
+coqc -Q SystemRF SystemRF -Q Denotations Denotations -R Bidirectional Bidirectional Bidirectional/Decidable.v
+echo "Checking SynthWFFT.v ..."
+coqc -Q SystemRF SystemRF -Q Denotations Denotations -R Bidirectional Bidirectional Bidirectional/SynthWFFT.v
+#echo "Checking SynthFType.v ..."
+#coqc -Q SystemRF SystemRF -Q Denotations Denotations -R Bidirectional Bidirectional Bidirectional/SynthFType.v
+#echo "Checking SynthWFType.v ..."
+#coqc -Q SystemRF SystemRF -Q Denotations Denotations -R Bidirectional Bidirectional Bidirectional/SynthWFType.v
+#echo "Checking SynthTyping.v ..."
+#coqc -Q SystemRF SystemRF -Q Denotations Denotations -R Bidirectional Bidirectional Bidirectional/SynthTyping.v
+
+#echo "Examples"
+#echo "Checking Abs.v"
+#coqc -Q SystemRF SystemRF -Q Denotations Denotations -R Examples Examples Examples/Abs.v
